icing/dopplerProgCompScript.sml
@@ -1,0 +1,128 @@
+(**
+  Icing benchmark input file
+  Use this file to run a CakeML AST through the Icing optimizer
+**)
+
+(* INCLUDES, do not change those *)
+open compilerTheory fromSexpTheory cfTacticsLib ml_translatorLib basis;
+open RealIntervalInferenceTheory ErrorIntervalInferenceTheory CertificateCheckerTheory;
+open source_to_sourceTheory CakeMLtoFloVerTheory CakeMLtoFloVerProofsTheory;
+open machine_ieeeTheory binary_ieeeTheory realTheory realLib RealArith;
+open preamble astToSexprLib;
+
+val _ = new_theory "dopplerProgComp";
+
+val _ = translation_extends "basisProg";
+
+(** Precondition **)
+val doppler_pre =
+“λ (x:(string,string) id).
+ if x = (Short "u")
+ then ((- 100/1, 100/1):real#real)
+ else if x = Short "v"
+ then (20/1, 20000/1)
+ else if x = Short "t"
+ then (- 30/1, 50/1)
+ else (0,0)”
+
+Definition doppler_pre_def:
+  doppler_pre = ^doppler_pre
+End
+
+(**
+  Define the CakeML source AST as a polyML/HOL4 declaration
+**)
+val doppler =
+“[Dlet unknown_loc (Pvar "doppler")
+  (Fun "u" (Fun "v" (Fun "t"
+  (** Numerical kernel **)
+  (FpOptimise Opt
+   (Let (SOME "t1")
+    (App (FP_bop FP_Add)
+     [
+       (App FpFromWord [Lit (Word64 (4644537666646730342w:word64))]);
+       (App (FP_bop FP_Mul)
+        [
+          (App FpFromWord [Lit (Word64 (4603579539098121011w:word64))]);
+          Var (Short  "t")
+        ])
+     ])
+    (App (FP_bop FP_Div)
+     [
+       (App (FP_bop FP_Mul)
+        [
+          (App (FP_uop FP_Neg)
+           [Var (Short "t1")]);
+          Var (Short "v")
+        ]);
+       (App (FP_bop FP_Mul)
+        [
+          (App (FP_bop FP_Add)
+           [Var (Short "t1");
+            Var (Short "u")]);
+          (App (FP_bop FP_Add)
+           [Var (Short "t1");
+            Var (Short "u")])
+        ])
+     ])
+   )))))]”
+
+Definition theAST_def:
+  theAST =
+  (** REPLACE AST BELOW THIS LINE **)
+  ^doppler
+End
+
+(** Optimizations to be applied by Icing **)
+Definition theOpts_def:
+  theOpts = extend_conf no_fp_opt_conf
+  [
+    (Binop FP_Add (Var 0) (Binop FP_Mul (Var 1) (Var 2)),
+     Binop FP_Add (Binop FP_Mul (Var 1) (Var 2)) (Var 0))
+    ;
+    (Binop FP_Add (Binop FP_Mul (Var 0) (Var 1)) (Var 2),
+    Terop FP_Fma (Var 2) (Var 0) (Var 1))
+    (*
+      (* WRITE OPTIMISATIONS HERE AS ; SEPARATED LIST *)
+    (Binop FP_Mul (Binop FP_Add (Var 0) (Var 1)) (Binop FP_Add (Var 0) (Var 1)),
+     Binop FP_Mul (Var 0) (Binop FP_Add (Var 1) (Var 1)));
+    (Binop FP_Mul (Var 0) (Binop FP_Add (Var 1) (Var 2)),
+     Terop FP_Fma (Var 0) (Var 1) (Var 2)) *)
+  ]
+End
+
+(** The code below stores in theorem theAST_opt the optimized version of the AST
+    from above and in errorbounds_AST the inferred FloVer roundoff error bounds
+ **)
+Theorem theAST_opt =
+  EVAL
+    (Parse.Term ‘
+      (source_to_source$no_opt_decs theOpts (source_to_source$stos_pass_decs theOpts
+       theAST))’);
+
+val doppler_opt = theAST_opt |> concl |> rhs;
+
+Definition theErrBound_def:
+  theErrBound = inv (2 pow (10))
+End
+
+Definition theProg_def:
+  theProg = ^doppler
+End
+
+Definition theOptProg_def:
+  theOptProg = ^doppler_opt
+End
+
+val _ = computeLib.del_funs [sptreeTheory.subspt_def];
+val _ = computeLib.add_funs [realTheory.REAL_INV_1OVER,
+                             binary_ieeeTheory.float_to_real_def,
+                             binary_ieeeTheory.float_tests,
+                             sptreeTheory.subspt_eq,
+                             sptreeTheory.lookup_def];
+
+Theorem errorbounds_AST =
+  EVAL (Parse.Term
+       ‘isOkError ^(concl theAST_opt |> rhs) ^doppler_pre theErrBound’);
+
+val _ = export_theory();
