icing/dopplerProofsScript.sml
@@ -1,0 +1,734 @@
+(**
+  Doppler program proofs
+**)
+
+open compilerTheory fromSexpTheory cfTacticsLib ml_translatorLib basis;
+open RealIntervalInferenceTheory ErrorIntervalInferenceTheory CertificateCheckerTheory;
+open source_to_sourceTheory CakeMLtoFloVerTheory CakeMLtoFloVerProofsTheory dopplerProgCompTheory;
+open machine_ieeeTheory binary_ieeeTheory realTheory realLib RealArith;
+open fromSexpTheory basis basis_ffiTheory cfHeapsBaseTheory;
+open preamble astToSexprLib;
+
+val _ = new_theory "dopplerProofs";
+
+val _ = translation_extends "basisProg";
+
+val printer =
+  “[Dlet unknown_loc (Pvar "printer")
+    (Fun "x"
+     (Let (SOME "z")
+      (App Opapp [
+         Var (Long "Word64" (Short "toInt"));
+         Var (Short "x")])
+      (Let (SOME "y")
+       (App Opapp [
+          Var (Long "Int" (Short "toString"));
+          Var (Short "z")])
+       (App Opapp [
+          Var (Long "TextIO" (Short "print"));
+          Var (Short "y")]))))]”;
+
+val _ = append_prog printer;
+
+val reader =
+“[Dlet unknown_loc (Pvar "reader")
+   (Fun "x"
+    (Let (SOME "inp")
+     (App Opapp [ Var (Long "TextIO" (Short "stdIn")); Con NONE []])
+     ( (Let (SOME "w1")
+         (App Opapp [
+            Var (Long "TextIO" (Short "inputLine"));
+            Var (Short "inp")])
+         (App Opapp [
+            Var (Long "Double" (Short "fromString"));
+            Var (Short "w1")])))))]”
+
+val _ = append_prog reader;
+
+val main =
+“[Dlet unknown_loc (Pvar "main")
+  (Fun "a"
+   (Let (SOME "d1")
+    (App FpFromWord [Lit (Word64 4607182418800017408w)])
+    (Let (SOME "d2")
+     (App FpFromWord [Lit (Word64 4607182418800017408w)])
+     (Let (SOME "d3")
+      (App FpFromWord [Lit (Word64 4607182418800017408w)])
+      (Let (SOME "x" )
+       (App Opapp [
+          App Opapp [
+            App Opapp [Var (Short "doppler"); Var (Short "d1")];
+            Var (Short "d2")];
+          Var (Short "d3")])
+       (Let (SOME "y")
+        (App FpToWord [Var (Short "x")])
+        (App Opapp [
+           Var (Short "printer");
+           Var (Short "y")])))))))]”;
+
+val iter_code = process_topdecs ‘
+ fun iter n s f =
+     if (n = 0) then s else iter (n-1) (f s) f;’
+
+val iter_count = “10000000:int”
+
+val call_code = Parse.Term ‘
+ [Dlet unknown_loc (Pvar "it")
+  (Let (SOME "b")
+   (Fun "x"
+    (Let NONE
+     (App Opapp [
+        App Opapp [
+          App Opapp [
+            Var (Short "doppler");
+            App FpFromWord [Lit (Word64 4607182418800017408w)]];
+          App FpFromWord [Lit (Word64 4607182418800017408w)]];
+        App FpFromWord [Lit (Word64 4607182418800017408w)]])
+     (Con NONE [])))
+   (Let (SOME "a") (Con NONE [])
+    (App Opapp [
+       App Opapp [
+         App Opapp [Var (Short "iter"); Lit (IntLit ^iter_count)];
+         Var (Short "a")]; Var (Short "b")])))]’;
+
+Definition theBenchmarkMain_def:
+  theBenchmarkMain =
+  (HD (^iter_code)) :: (^call_code)
+End
+
+val st_no_doppler = get_ml_prog_state ();
+
+val doppler_env = st_no_doppler
+  |> ml_progLib.clean_state
+  |> ml_progLib.remove_snocs
+  |> ml_progLib.get_env;
+
+val _ = append_prog (theOptProg_def |> concl |> rhs)
+
+val _ = append_prog main;
+
+val st = get_ml_prog_state ();
+
+(*
+val benchmarking = false;
+
+val fullProg =
+  if benchmarking
+  then
+    (EVAL (Parse.Term
+           ‘(^(theAST_def |> concl |> rhs)) :: (^(theBenchmarkMain_def |> concl |> rhs))’)
+     |> concl |> rhs)
+  else
+    (EVAL (Parse.Term
+           ‘[HD (^(theAST_def |> concl |> rhs)); HD ^main]’)
+     |> concl |> rhs);
+
+val fullOptProg =
+  if benchmarking
+  then
+    (EVAL (Parse.Term ‘(HD (^(theAST_opt |> concl |> rhs))) :: (^(theBenchmarkMain_def |> concl |> rhs))’)
+     |> concl |> rhs)
+  else
+    (EVAL (Parse.Term
+           ‘[HD (^(theAST_opt |> concl |> rhs)); HD ^main]’)
+     |> concl |> rhs);
+
+val filename = "theProg.sexp.cml";
+val _ = ((write_ast_to_file filename) o rhs o concl) theProg_def;
+
+val filename = "theOptProg.sexp.cml";
+val _ = ((write_ast_to_file filename) o rhs o concl) theOptProg_def;
+*)
+
+Definition getDeclLetParts_def:
+  getDeclLetParts [Dlet loc (Pvar fname) e] =
+  let (vars, body) = stripFuns e in
+  (fname, vars, body)
+End
+
+Definition doppler_opt_real_spec_def:
+  doppler_opt_real_spec decl =
+  let (fname, fvars, body) = getDeclLetParts decl in
+  (λ w1.
+   λ w2.
+   λ w3.
+   case evaluate
+     (empty_state with fp_state := empty_state.fp_state with real_sem := T)
+     (^doppler_env with v := toRspace (extend_env_with_vars (REVERSE fvars) (REVERSE [w1;w2;w3]) ^(doppler_env).v))
+   [realify body] of
+   | (st, Rval [Real r]) => r)
+End
+
+Definition doppler_opt_float_spec_def:
+  doppler_opt_float_spec decl =
+  let (fname, fvars, body) = getDeclLetParts decl in
+  (λ w1.
+   λ w2.
+   λ w3.
+   case evaluate empty_state
+   (^doppler_env with v := extend_env_with_vars (REVERSE fvars) (REVERSE [w1;w2;w3]) ^(doppler_env).v)
+   [body] of
+   | (st, Rval [FP_WordTree fp]) => fp)
+End
+
+(** SPECIFICATION THEOREM FOR Doppler **)
+Definition DOUBLE_def:
+  DOUBLE (d:fp_word_val) =
+  λ v. v = FP_WordTree d
+End
+
+(*
+Definition DOUBLE_APPROX_def:
+  DOUBLE_APPROX (r:real) (fp:fp_word_val) (err:real) =
+  λ v.
+  case v of
+  |FP_WordTree fp2 => (compress_word fp2 = compress_word fp ∧
+                      real$abs(fp64_to_real (compress_word fp) - r) ≤ err)
+  | _ => F
+End
+*)
+
+val (fname, fvars, body) =
+  EVAL (Parse.Term ‘getDeclLetParts ^(theOptProg_def |> concl |> rhs)’)
+  |> concl |> rhs |> dest_pair
+  |> (fn (x,y) => let val (y,z) = dest_pair y in (x,y,z) end)
+
+Theorem printer_spec:
+  WORD (w:word64) v ⇒
+  app (p:'ffi ffi_proj) ^(fetch_v "printer" st)
+    [v]
+    (STDIO fs)
+    (POSTv uv. &UNIT_TYPE () uv * STDIO (add_stdout fs (mlint$toString (&w2n w))))
+Proof
+  xcf "printer" st
+  \\ xlet_auto
+  >- (xsimpl)
+  \\ xlet_auto
+  >- (xsimpl)
+  \\ xapp \\ xsimpl
+QED
+
+(**  INSTREAM fd fdv ∧ IS_SOME (get_file_content fs fd) ∧ get_mode fs fd = SOME ReadMode
+   ⇒
+   app (p:'ffi ffi_proj) TextIO_inputLine_v [fdv]
+     (STDIO fs)
+     (POSTv sov.
+       &OPTION_TYPE STRING_TYPE (OPTION_MAP implode (lineFD fs fd)) sov *
+       STDIO (lineForwardFD fs fd))
+Theorem reader_spec:
+app (p:ffi ffi_proj) ^(fetch_v "reader" st)
+  [Conv NONE []]
+  (STDIO fs)
+  (POSTv uv. &(DOUBLE d uv))
+Proof
+  xcf "reader" st
+  \\ xlet_auto
+  \\ assume_tac TextIOProofTheory.INSTREAM_stdin
+  \\ xlet ‘POSTv sov.
+       &OPTION_TYPE STRING_TYPE (OPTION_MAP implode (lineFD fs 0)) sov *
+       STDIO (lineForwardFD fs 0)’
+  \\ xlet_auto
+  \\ xlet ‘POSTv uv. INSTREAM 0 stdin_v uv’
+  \\ xlet_auto
+**)
+
+Theorem cf_fpfromword:
+  ∀ env.
+  cf_fpfromword (Lit (Word64 w)) env (STDIO fs)
+  (POSTv v. &DOUBLE (Fp_const w) v * STDIO fs)
+Proof
+  rpt strip_tac
+  \\ qmatch_goalsub_abbrev_tac ‘cf_fpfromword _ _ _ Post’
+  \\ fs[cf_fpfromword_def, cfHeapsTheory.local_def, cfNormaliseTheory.exp2v_def,
+         cfTheory.app_fpfromword_def]
+  \\ rpt strip_tac
+  \\ qexists_tac ‘STDIO fs’ \\ qexists_tac ‘emp’
+  \\ qexists_tac ‘Post’ \\ rpt conj_tac \\ unabbrev_all_tac \\ xsimpl
+   >- (
+    simp[set_sepTheory.STAR_def] \\ qexists_tac ‘h’ \\ qexists_tac ‘EMPTY’
+    \\ fs[SPLIT_def, emp_def])
+   \\ fs[DOUBLE_def, set_sepTheory.SEP_IMP_def]
+   \\ rpt strip_tac \\ fs[set_sepTheory.cond_def, set_sepTheory.STAR_def]
+   \\ unabbrev_all_tac \\ fs[SPLIT_def]
+QED
+
+val doppler_opt = theAST_opt |> concl |> rhs;
+
+(*
+val _ = computeLib.del_funs [sptreeTheory.subspt_def];
+val _ = computeLib.add_funs [realTheory.REAL_INV_1OVER,
+                             binary_ieeeTheory.float_to_real_def,
+                             binary_ieeeTheory.float_tests,
+                             sptreeTheory.subspt_eq,
+                             sptreeTheory.lookup_def];
+*)
+
+val doppler_pre = doppler_pre_def |> concl |> rhs;
+
+Definition doppler_side_def:
+  doppler_side w1 w2 w3 =
+   (evaluate_fine empty_state
+     (^doppler_env with v :=
+      extend_env_with_vars (REVERSE ^fvars) (REVERSE [w1;w2;w3]) ^(doppler_env).v)
+     [^body] ∧
+     (is_precond_sound ^fvars [w1; w2; w3] ^doppler_pre))
+End
+
+Definition doppler_float_result_def:
+  doppler_float_result w1 w2 w3 =
+    (compress_word (doppler_opt_float_spec ^doppler_opt w1 w2 w3))
+End
+
+Definition doppler_real_result_def:
+  doppler_real_result w1 w2 w3 =
+    (doppler_opt_real_spec ^doppler_opt w1 w2 w3)
+End
+
+Definition doppler_satisfies_error_def:
+  doppler_satisfies_error w1 w2 w3 eps =
+    (∃ r. doppler_opt_real_spec ^doppler_opt w1 w2 w3 = r ∧
+    real$abs (
+      fp64_to_real (compress_word (doppler_opt_float_spec ^doppler_opt w1 w2 w3)) -
+      r) ≤ eps)
+End
+
+Theorem doppler_spec:
+  doppler_side w1 w2 w3 ∧
+  DOUBLE (Fp_const w1) d1 ∧
+  DOUBLE (Fp_const w2) d2 ∧
+  DOUBLE (Fp_const w3) d3 ⇒
+  let theResult = (doppler_opt_float_spec ^doppler_opt w1 w2 w3) in
+  app (p:'ffi ffi_proj) ^(fetch_v "doppler" st)
+    [d1; d2; d3]
+    (emp)
+    (POSTv v.
+     &DOUBLE theResult v) ∧
+  real$abs (fp64_to_real (doppler_float_result w1 w2 w3) - doppler_real_result w1 w2 w3) ≤ theErrBound
+Proof
+  rpt gen_tac \\ simp[app_def, doppler_side_def, doppler_real_result_def, doppler_float_result_def]
+  \\ rpt (disch_then assume_tac)
+  \\ simp[app_basic_def, getDeclLetParts_def, stripFuns_def, PULL_FORALL]
+  \\ rpt (gen_tac ORELSE (disch_then assume_tac)) \\ fs[]
+  \\ qpat_x_assum ‘evaluate_fine _ _ _’ mp_tac
+  \\ qmatch_goalsub_abbrev_tac ‘evaluate_fine empty_state _ [doppler_body]’
+  \\ disch_then assume_tac
+  \\ mp_tac errorbounds_AST
+  \\ fs[isOkError_def, option_case_eq, pair_case_eq, getErrorbounds_def, stripFuns_def, PULL_EXISTS]
+  \\ TOP_CASE_TAC \\ fs[option_case_eq, pair_case_eq]
+  \\ TOP_CASE_TAC \\ fs[option_case_eq, pair_case_eq]
+  \\ TOP_CASE_TAC \\ fs[option_case_eq, pair_case_eq]
+  \\ rpt (gen_tac ORELSE (disch_then assume_tac)) \\ fs[] \\ rveq
+  \\ first_assum (mp_then Any mp_tac (INST_TYPE [“:'ffi” |-> “:unit”] CakeML_FloVer_infer_error))
+  \\ disch_then (qspec_then ‘empty_state’ mp_tac) \\ fs[]
+  \\ disch_then (qspecl_then
+                 [‘merge_env dopplerProofs_env_0 init_env’,
+                  ‘[Short "u"; Short "v"; Short "t"]’,
+                  ‘[w1;w2;w3]’,
+                  ‘Fun "u" (Fun "v" (Fun "t" (FpOptimise NoOpt e)))’,
+                  ‘(FpOptimise NoOpt e)’]  mp_tac)
+  \\ fs[]
+  \\ rpt (disch_then drule)
+  \\ impl_tac >- (unabbrev_all_tac \\ fs[stripFuns_def])
+  \\ rpt (disch_then assume_tac) \\ fs[]
+  \\ reverse conj_tac
+  >- (
+   fs[doppler_opt_float_spec_def, doppler_opt_real_spec_def]
+   \\ simp[getDeclLetParts_def] \\ rewrite_tac[stripFuns_def]
+   \\ rpt (pop_assum mp_tac)
+   \\ simp[]
+   \\ rpt strip_tac \\ irule REAL_LE_TRANS \\ asm_exists_tac \\ fs[])
+  \\ rpt strip_tac
+  \\ simp[semanticPrimitivesTheory.do_opapp_def, fetch "-" "doppler_v_def"]
+  \\ Q.REFINE_EXISTS_TAC ‘Val v’
+  \\ simp[evaluate_to_heap_def, evaluate_ck_def, terminationTheory.evaluate_def]
+  \\ qexists_tac ‘EMPTY’ \\ qexists_tac ‘EMPTY’
+  \\ fs[emp_def, set_sepTheory.SPLIT_def, cfHeapsBaseTheory.SPLIT3_def]
+  \\ simp[set_sepTheory.SEP_EXISTS]
+  \\ qexists_tac ‘emp’ \\ simp[set_sepTheory.STAR_def]
+  \\ ntac 2 (qexists_tac ‘EMPTY’)
+  \\ fs[emp_def, set_sepTheory.SPLIT_def, cfHeapsBaseTheory.SPLIT3_def]
+  \\ simp[set_sepTheory.cond_def]
+  \\ rpt strip_tac
+  \\ Q.REFINE_EXISTS_TAC ‘Val v’ \\ simp[]
+  \\ ntac 2 (qexists_tac ‘EMPTY’) \\ rpt conj_tac \\ TRY (simp[DISJOINT_DEF] \\ NO_TAC)
+  \\ qexists_tac ‘emp’ \\ simp[emp_def]
+  \\ rpt strip_tac
+  \\ Q.REFINE_EXISTS_TAC ‘Val v’ \\ simp[]
+  \\ ‘DISJOINT (st2heap p st'') EMPTY’ by (simp[DISJOINT_DEF])
+  \\ asm_exists_tac \\ simp[DOUBLE_def]
+  \\ mp_tac (GEN_ALL (SIMP_RULE std_ss [ml_progTheory.eval_rel_def] evaluate_empty_state_IMP))
+  \\ disch_then (qspecl_then [‘FP_WordTree fp2’, ‘st''’, ‘st''.refs’, ‘FpOptimise NoOpt e’] mp_tac)
+  \\ fs[semanticPrimitivesTheory.state_component_equality, empty_state_def, PULL_EXISTS]
+  \\ qmatch_goalsub_abbrev_tac ‘evaluate _ dEnv _ = _’
+  \\ disch_then (qspecl_then [‘dEnv’, ‘0’, ‘0’] mp_tac)
+  \\ impl_tac
+  >- (fs[] \\ cheat (* FIX CakeML_FloVer_thm *))
+  \\ strip_tac \\ qexists_tac ‘ck1’
+  \\ fs[doppler_opt_float_spec_def, getDeclLetParts_def, stripFuns_def, empty_state_def]
+  \\ fs[cfStoreTheory.st2heap_def]
+  \\ cheat (* FIXME: Minor ref juggling *)
+QED
+
+Theorem main_spec:
+  ∀ p.
+  doppler_side 4607182418800017408w 4607182418800017408w 4607182418800017408w ⇒
+  app (p:'ffi ffi_proj) ^(fetch_v "main" st)
+    [Conv NONE []]
+    (STDIO fs)
+    (POSTv uv. &UNIT_TYPE () uv *
+     STDIO (add_stdout fs (mlint$toString (&w2n (compress_word (doppler_opt_float_spec ^doppler_opt 4607182418800017408w 4607182418800017408w 4607182418800017408w))))))
+    ∧
+    real$abs (fp64_to_real (doppler_float_result 4607182418800017408w 4607182418800017408w 4607182418800017408w) - doppler_real_result 4607182418800017408w 4607182418800017408w 4607182418800017408w) ≤ theErrBound
+Proof
+  rpt strip_tac
+  \\ first_x_assum (mp_then Any assume_tac (SIMP_RULE std_ss [] doppler_spec))
+  >- (
+   xcf "main" st
+   \\ xlet ‘POSTv v. &(DOUBLE (Fp_const 4607182418800017408w) v) * STDIO fs’
+   >- (irule cf_fpfromword)
+   \\ xlet ‘POSTv v. &(DOUBLE (Fp_const 4607182418800017408w) v) * STDIO fs’
+   >- (irule cf_fpfromword)
+   \\ xlet ‘POSTv v. &(DOUBLE (Fp_const 4607182418800017408w) v) * STDIO fs’
+   >- (irule cf_fpfromword)
+   \\ first_x_assum (qspecl_then [‘p’, ‘v''’, ‘v'’, ‘v’] mp_tac)
+   \\ impl_tac \\ fs[] \\ strip_tac
+   \\ xlet_auto >- xsimpl
+   \\ fs[DOUBLE_def]
+   \\ Cases_on ‘v'3'’ \\ fs[]
+   \\ xlet ‘POSTv v. &WORD (compress_word f) v * STDIO fs’
+   >- (
+    fs[cf_fptoword_def, cfHeapsTheory.local_def, cfNormaliseTheory.exp2v_def,
+       cfTheory.app_fptoword_def]
+    \\ rpt strip_tac
+    \\ fs[WORD_def]
+    \\ qexists_tac ‘STDIO fs’ \\ qexists_tac ‘emp’
+    \\ simp[]
+    \\ qexists_tac ‘POSTv v. &WORD (compress_word f) v * STDIO fs’ \\ rpt conj_tac
+    >- (
+     simp[set_sepTheory.STAR_def] \\ qexists_tac ‘h’ \\ qexists_tac ‘EMPTY’
+     \\ fs[SPLIT_def, emp_def])
+    >- (
+     fs[DOUBLE_def, set_sepTheory.SEP_IMP_def]
+     \\ rpt strip_tac \\ fs[set_sepTheory.cond_def, set_sepTheory.STAR_def]
+     >- (qexists_tac ‘s’ \\ fs[SPLIT_def])
+     \\ xsimpl)
+    \\ xsimpl \\ rveq \\ strip_tac \\ fs[WORD_def, DOUBLE_def])
+   \\ xapp \\ xsimpl)
+  \\ fs[DOUBLE_def]
+QED
+
+Definition u_val_def:
+  u_val = 4607182418800017408w
+End
+
+Definition v_val_def:
+  v_val = 4607182418800017408w
+End
+
+Definition t_val_def:
+  t_val = 4607182418800017408w
+End
+
+Theorem main_whole_prog_spec:
+  doppler_side u_val v_val t_val ⇒
+  whole_prog_spec ^(fetch_v "main" st) cl fs
+  NONE
+  ((=)
+   (add_stdout fs (mlint$toString (&w2n (compress_word (doppler_opt_float_spec ^doppler_opt u_val v_val t_val))))))
+  ∧
+    real$abs (fp64_to_real (doppler_float_result u_val v_val t_val) - doppler_real_result u_val v_val t_val) ≤ theErrBound
+Proof
+  simp[whole_prog_spec_def, u_val_def, v_val_def, t_val_def]
+  \\ qmatch_goalsub_abbrev_tac`fs1 = _ with numchars := _`
+  \\ rpt (strip_tac)
+  \\ qspec_then ‘(basis_proj1, basis_proj2)’ mp_tac main_spec
+  \\ impl_tac \\ fs[]
+  \\ strip_tac
+  \\ qexists_tac`fs1`
+  \\ simp[Abbr`fs1`,GSYM add_stdo_with_numchars,with_same_numchars]
+  \\ first_x_assum (fn main_spec => irule (MP_CANON (MATCH_MP app_wgframe main_spec)))
+  \\ xsimpl
+QED
+
+val spec = main_whole_prog_spec;
+val name = "main";
+
+(** TODO: Below copied from basis_ffiLib.sml because of a bug in subset_basis_st *)
+
+val basis_ffi_const = prim_mk_const{Thy="basis_ffi",Name="basis_ffi"};
+val basis_ffi_tm =
+  list_mk_comb(basis_ffi_const,
+    map mk_var
+      (zip ["cl","fs"]
+        (#1(strip_fun(type_of basis_ffi_const)))))
+
+local
+  val heap_thms = [COMMANDLINE_precond, STDIO_precond];
+  val heap_thms2 = [COMMANDLINE_precond, STDIO_precond, RUNTIME_precond];
+  val user_thms = ref ([]: thm list);
+  fun build_set [] = raise(ERR"subset_basis_st""no STDOUT in precondition")
+    | build_set [th] = th
+    | build_set (th1::th2::ths) =
+        let
+          val th = MATCH_MP append_hprop (CONJ th1 th2)
+          val th = CONV_RULE(LAND_CONV EVAL)th
+          val th = MATCH_MP th TRUTH |> SIMP_RULE (srw_ss()) [UNION_EMPTY]
+          val th = (CONV_RULE(RAND_CONV (pred_setLib.UNION_CONV EVAL)) th
+          handle _ => th) (* TODO quick fix *)
+        in build_set (th::ths) end
+in
+  fun add_user_heap_thm thm =
+      (user_thms := thm :: (!user_thms);
+       HOL_MESG ("Adding user heap theorem:\n" ^ thm_to_string thm ^ "\n"))
+  val sets_thm2 = build_set heap_thms2;
+  val sets2 = rand (concl sets_thm2)
+  fun mk_user_sets_thm () = build_set (heap_thms @ (!user_thms))
+end
+
+val (whole_prog_spec_thm,sets,sets_thm) =
+let
+  val sets_thm = mk_user_sets_thm ()
+  val sets     = rand (concl sets_thm)
+in
+  (whole_prog_spec_semantics_prog, sets, sets_thm)
+end
+
+(** Build intermediate theorem with SPLIT assumption **)
+val th =
+  whole_prog_spec_thm
+  |> C MATCH_MP (st |> get_Decls_thm |> GEN_ALL |> ISPEC basis_ffi_tm)
+  |> SPEC(stringSyntax.fromMLstring name)
+  |> CONV_RULE(QUANT_CONV(LAND_CONV(LAND_CONV EVAL THENC SIMP_CONV std_ss [])))
+  |> CONV_RULE(HO_REWR_CONV UNWIND_FORALL_THM1)
+  |> C HO_MATCH_MP (CONJUNCT1 (UNDISCH_ALL spec))
+  |> SIMP_RULE bool_ss [option_case_def, set_sepTheory.SEP_CLAUSES]
+
+val prog_with_snoc = th |> concl |> find_term listSyntax.is_snoc
+val prog_rewrite = EVAL prog_with_snoc
+val th = PURE_REWRITE_RULE[prog_rewrite] th
+val (split,precondh1) = th |> concl |> dest_imp |> #1 |> strip_exists |> #2 |> dest_conj
+val precond = rator precondh1
+val st = split |> rator |> rand
+
+(*This tactic proves that for a given state, parts_ok holds for the ffi and the basis_proj2*)
+val prove_parts_ok_st =
+    qmatch_goalsub_abbrev_tac`st.ffi`
+    \\ `st.ffi.oracle = basis_ffi_oracle`
+    by( simp[Abbr`st`] \\ EVAL_TAC \\ NO_TAC)
+    \\ rw[cfStoreTheory.parts_ok_def]
+    \\ TRY ( simp[Abbr`st`] \\ EVAL_TAC \\ NO_TAC )
+    \\ TRY ( imp_res_tac oracle_parts \\ rfs[] \\ NO_TAC)
+    \\ qpat_x_assum`MEM _ basis_proj2`mp_tac
+    \\ simp[basis_proj2_def,basis_ffi_part_defs,cfHeapsBaseTheory.mk_proj2_def]
+    \\ TRY (qpat_x_assum`_ = SOME _`mp_tac)
+    \\ simp[basis_proj1_def,basis_ffi_part_defs,cfHeapsBaseTheory.mk_proj1_def,FUPDATE_LIST_THM]
+    \\ rw[] \\ rw[] \\ pairarg_tac \\ fs[FLOOKUP_UPDATE] \\ rw[]
+    \\ fs[FAPPLY_FUPDATE_THM,cfHeapsBaseTheory.mk_ffi_next_def]
+    \\ TRY PURE_FULL_CASE_TAC
+    \\ fs[]
+    \\ EVERY (map imp_res_tac (CONJUNCTS basis_ffi_length_thms))
+    \\ fs[fs_ffi_no_ffi_div,cl_ffi_no_ffi_div]
+    \\ srw_tac[DNF_ss][] \\ simp[basis_ffi_oracle_def];
+
+val SPLIT_thm =
+  let
+    val to_inst = free_vars sets
+    val goal = pred_setSyntax.mk_subset(sets,st)
+    val tac = (
+          fs[cfStoreTheory.st2heap_def, cfStoreTheory.FFI_part_NOT_IN_store2heap,
+             cfStoreTheory.Mem_NOT_IN_ffi2heap, cfStoreTheory.ffi2heap_def]
+       \\ qmatch_goalsub_abbrev_tac`parts_ok ffii (basis_proj1,basis_proj2)`
+       \\ `parts_ok ffii (basis_proj1,basis_proj2)`
+              by (fs[Abbr`ffii`] \\ prove_parts_ok_st)
+       \\ fs[Abbr`ffii`]
+       \\ EVAL_TAC
+       \\ rw[cfAppTheory.store2heap_aux_append_many,INJ_MAP_EQ_IFF,INJ_DEF,FLOOKUP_UPDATE]
+       \\ rw[cfStoreTheory.store2heap_aux_def]
+       )
+    val (subgoals,_) = tac ([],goal)
+    fun mk_mapping (x,y) =
+      if tmem x to_inst then SOME (x |-> y) else
+      if tmem y to_inst then SOME (y |-> x) else NONE
+    fun safe_dest_eq tm =
+      if boolSyntax.is_eq tm then boolSyntax.dest_eq tm else
+      Lib.tryfind boolSyntax.dest_eq (boolSyntax.strip_disj tm)
+      handle HOL_ERR _ =>
+        raise(ERR"subset_basis_st"("Could not prove heap subgoal: "^(Parse.term_to_string tm)))
+    val s =
+       List.mapPartial (mk_mapping o safe_dest_eq o #2) subgoals
+    val goal' = Term.subst s goal
+    val th = prove(goal',tac)
+    val th =
+        MATCH_MP SPLIT_exists (CONJ (INST s sets_thm) th)
+    val length_hyps = mapfilter (assert listSyntax.is_length o lhs) (hyp th)
+                   |> map EVAL
+  in
+    foldl (uncurry PROVE_HYP) th length_hyps
+  end;
+
+val semantics_prog_thm =
+  MATCH_MP th SPLIT_thm
+  |> DISCH_ALL
+  |> REWRITE_RULE [AND_IMP_INTRO]
+  |> CONV_RULE ((RATOR_CONV o RAND_CONV) (SIMP_CONV std_ss [LENGTH]))
+  |> REWRITE_RULE [GSYM AND_IMP_INTRO]
+  |> UNDISCH_ALL
+
+val doppler_prog_tm = rhs (concl prog_rewrite);
+
+val doppler_prog_def = Define`doppler_prog = ^doppler_prog_tm`;
+
+Theorem IMP_SPLIT:
+  (P ⇒ (Q1 ∧ Q2)) ⇔ ((P ⇒ Q1) ∧ (P ⇒ Q2))
+Proof
+  EQ_TAC \\ rpt strip_tac \\ fs[]
+QED
+
+val full_semantics_prog_thm =
+  LIST_CONJ [
+    DISCH_ALL semantics_prog_thm,
+    CONJUNCT2 (SIMP_RULE std_ss [IMP_SPLIT] main_whole_prog_spec) |> ONCE_REWRITE_RULE [CONJ_COMM]
+  ]
+  |> SIMP_RULE std_ss [GSYM AND_IMP_INTRO]
+  |> SIMP_RULE std_ss [GSYM IMP_SPLIT];
+
+Theorem doppler_semantics =
+  full_semantics_prog_thm |> ONCE_REWRITE_RULE[GSYM doppler_prog_def]
+  |> DISCH_ALL |> SIMP_RULE std_ss [AND_IMP_INTRO,GSYM CONJ_ASSOC];
+
+Theorem doppler_semantics_final:
+  doppler_side u_val v_val t_val ⇒
+     (wfcl cl ∧ wfFS fs ∧ STD_streams fs ⇒
+      ∃io_events (w:word64).
+          semantics_prog (init_state (basis_ffi cl fs)) init_env doppler_prog
+            (Terminate Success io_events) ∧
+          extract_fs fs io_events =
+          SOME
+            (add_stdout fs (toString:int->mlstring (&((w2n w):num)))) ∧
+     doppler_float_result u_val v_val t_val = w) ∧
+     real$abs (fp64_to_real (doppler_float_result u_val v_val t_val) - doppler_real_result u_val v_val t_val) ≤ theErrBound
+Proof
+  rpt strip_tac
+  \\ imp_res_tac doppler_semantics \\ fs[]
+  \\ asm_exists_tac \\ fs[doppler_float_result_def]
+QED
+
+(**
+FINAL THEOREM:
+
+Let Doppler be the following program ... using floating-point operations,
+let DopplerReal be to_real(Doppler), where to_real syntactically replaces all
+floating-point operations by their real-numbered counterparts, and let
+DopplerOpt = optimise(Doppler, ids), where optimise syntactically transforms a
+floating-point program using our optimisation algorithm with identities ids, and
+suppose ids contains only real-valued identities.
+Then if there is a real number r such that
+real_semantics(DopplerReal) = print(r), then there is a floating-point word w
+such that semantics(DopplerOpt) = print(w), and |real(w)-r| ≤ error(DopplerOpt) ≤ the user given error constraint ε
+(with respect to DopplerReal), where error uses the FloVer analysis tool to
+compute an upper bound on the worst-case roundoff error between DopplerReal and DopplerOpt.
+
+or
+
+Let DopplerReal be the following program ... that uses real-number operations,
+let Doppler be floatify(DopplerReal), where floatify syntactically turns all
+real-number operations into floating-point operations, and let
+DopplerOpt = optimise(Doppler, ids), where optimise syntactically transforms a
+floating-point program using our optimisation algorithm with identities ids, and
+suppose ids contains only real-valued identities.
+Then if there is a real number r such that
+real_semantics(DopplerReal) = print(r), then there is a floating-point word w
+such that semantics(DopplerOpt) = print(w), and |real(w)-r| < error(DopplerReal),
+where error uses the FloVer analysis tool to compute an upper bound on the
+worst-case roundoff error between DopplerReal and DopplerOpt.
+**)
+
+(**
+Definition semantics_adds_to_stdout_def:
+  semantics_adds_to_stdout cl fs prog str =
+    ∃ io_events.
+      semantics_prog (init_state (basis_ffi cl fs)) init_env prog
+        (Terminate Success io_events) ∧
+      extract_fs fs io_events = SOME (add_stdout fs str)
+End
+
+Theorem doppler_kernel_main_thm:
+  wfcl cl ∧ wfFS fs ∧ STD_streams fs ⇒
+  ∃ (w:word64) (r:real).
+    semantics_adds_to_stdout cl fs theOptProg
+      (word64_to_string w) ∧
+    semantics_adds_to_stdout cl fs (realify theProg)
+      (real_to_string r) ∧
+    real$abs(fp64_to_real w - r) ≤ theErrBound
+Proof
+  rpt strip_tac
+  (* TODO: By computation above... *)
+  \\ assume_tac (Q.prove (‘isOkError theAST theErrBound = SOME T’, cheat))
+  \\ simp[Once theOptProg_def]
+  \\ simp[Once semanticsTheory.semantics_prog_def,
+          semanticsTheory.evaluate_prog_with_clock_def,
+          Once evaluatePropsTheory.evaluate_decs_cons]
+  (* Rewrite with eval theorem *)
+  \\ simp[Once theAST_opt_eval]
+  \\ simp[Once semanticPrimitivesTheory.extend_dec_env_def]
+  \\ simp[ml_progTheory.init_state_def]
+  \\ simp[terminationTheory.evaluate_decs_def]
+  \\ simp[ALL_DISTINCT, astTheory.pat_bindings_def]
+  \\ simp[Once terminationTheory.evaluate_def]
+  \\ simp[Once terminationTheory.evaluate_def]
+  \\ simp[astTheory.getOpClass_def]
+  \\ simp[Once evaluatePropsTheory.evaluate_cons, evaluate_fpfromword_const]
+  \\ simp[Once terminationTheory.evaluate_def]
+  \\ simp[astTheory.getOpClass_def, Once evaluatePropsTheory.evaluate_cons, evaluate_fpfromword_const]
+  \\ simp[Once terminationTheory.evaluate_def]
+  \\ simp[astTheory.getOpClass_def, Once evaluatePropsTheory.evaluate_cons, evaluate_fpfromword_const]
+  \\ simp[Once terminationTheory.evaluate_def]
+  \\ qmatch_goalsub_abbrev_tac ‘<| v := Bind [("doppler", Closure init_env "u" doppler_body)] []; c := Bind [] []|>’
+  \\ simp[ml_progTheory.nsLookup_nsAppend_Short, namespaceTheory.nsLookup_def]
+  \\ simp[semanticPrimitivesTheory.do_opapp_def]
+  \\ fs[GSYM PULL_EXISTS]
+  \\ simp[PULL_EXISTS]
+  \\ qexists_tac ‘5’ \\ fs[evaluateTheory.dec_clock_def]
+  \\ unabbrev_all_tac \\ simp[Once terminationTheory.evaluate_def]
+  \\ simp[Once terminationTheory.evaluate_def]
+  \\ qmatch_goalsub_abbrev_tac ‘Let NONE (App Opapp [Var (Long "Runtime" (Short "assert")); doppler_pre ]) _’
+  \\ simp[Once terminationTheory.evaluate_def]
+  \\ qmatch_goalsub_abbrev_tac ‘evaluate stA envA [App Opapp [Var (Long "Runtime" (Short "assert")); doppler_pre]]’
+  \\ ‘evaluate stA envA [App Opapp [Var (Long "Runtime" (Short "assert")); doppler_pre]] = (dec_clock stA, Rval [Conv NONE []])’
+     by (cheat)
+  \\ fs[]
+  \\ simp[Once terminationTheory.evaluate_def]
+  \\ unabbrev_all_tac \\ fs[evaluateTheory.dec_clock_def]
+  \\ qmatch_goalsub_abbrev_tac ‘combine_dec_result <| v := Bind [doppler_clos] _; c := _ |>’
+  \\ qmatch_goalsub_abbrev_tac ‘evaluate stA envA [doppler_body]’
+
+  \\ fs[isOkError_def, option_case_eq, pair_case_eq, getErrorbounds_def]
+  \\ rveq
+  \\ qspecl_then [‘stA’, ‘stA’,‘envA’, ‘prepareGamma floverVars’, ‘P’, ‘theBounds’,
+                  ‘theAST’, ‘ids’, ‘cake_P’, ‘f’, ‘floverVars’, ‘varMap’,
+                  ‘freshId’, ‘freshId'’, ‘theIds’, ‘theCmd’, ‘dVars’]
+                 mp_tac CakeML_FloVer_infer_error
+  \\ impl_tac \\ fs[]
+  >- (
+   rpt conj_tac
+   >- (cheat) (* TODO: Should become a different assumption *)
+   >- (cheat) (* Same as above *)
+   >- (cheat) (* reword to :st.fp_state.canOpt ≠ FPScope Opt *)
+   >- (cheat) (* Assumption *)
+   >- (cheat) (* Lemma *)
+   >- (cheat) (* Assumption? *)
+   )
+  \\ strip_tac
+  \\ ‘doppler_body = f’ by (cheat)
+  \\ fs[]
+  \\
+
+       TextIOProofTheory.print_spec
+       IntProofTheory.toString_spec
+
+
+
+QED
+*)
+
+val _ = export_theory();
